src/program_proof/mvcc/wrbuf_open_tuples.v
@@ -1,0 +1,73 @@
+From Perennial.program_proof.mvcc Require Import
+     wrbuf_prelude wrbuf_repr
+     index_proof
+     tuple_repr tuple_own tuple_free tuple_write_lock.
+
+Section heap.
+Context `{!heapGS Σ, !mvcc_ghostG Σ}.
+
+(*********************************************************************)
+(* func (wrbuf *WrBuf) OpenTuples(tid uint64, idx *index.Index) bool *)
+(*********************************************************************)
+Theorem wp_wrbuf__OpenTuples wrbuf (tid : u64) (idx : loc) m γ :
+  {{{ own_wrbuf_xtpls wrbuf m }}}
+    WrBuf__OpenTuples #wrbuf #tid #idx
+  {{{ (ok : bool) (tpls : gmap u64 loc), RET #ok;
+      own_wrbuf wrbuf m tpls ∗ own_tuples_locked (int.nat tid) tpls γ
+  }}}.
+Proof.
+  iIntros (Φ) "Hwrbuf HΦ".
+  wp_call.
+  iNamed "Hwrbuf".
+  
+  (***********************************************************)
+  (* ents := wrbuf.ents                                      *)
+  (* var pos uint64 = 0                                      *)
+  (* for pos < uint64(len(ents)) {                           *)
+  (*     ent := ents[pos]                                    *)
+  (*     tpl := idx.GetTuple(ent.key)                        *)
+  (*     ents[pos] = WrEnt {                                 *)
+  (*         key : ent.key,                                  *)
+  (*         val : ent.val,                                  *)
+  (*         wr  : ent.wr,                                   *)
+  (*         tpl : tpl,                                      *)
+  (*     }                                                   *)
+  (*     ret := tpl.Own(tid)                                 *)
+  (*     if ret != common.RET_SUCCESS {                      *)
+  (*         break                                           *)
+  (*     }                                                   *)
+  (*     pos++                                               *)
+  (* }                                                       *)
+  (***********************************************************)
+
+  (**
+   * Get [mods_token] and [is_tuple] for each element in [ents].
+   *)
+
+  (***********************************************************)
+  (* if pos < uint64(len(ents)) {                            *)
+  (*     var i uint64 = 0                                    *)
+  (*     for i < pos {                                       *)
+  (*         tpl := ents[i].tpl                              *)
+  (*         tpl.Free()                                      *)
+  (*         i++                                             *)
+  (*     }                                                   *)
+  (*     return false                                        *)
+  (* }                                                       *)
+  (***********************************************************)
+
+  (***********************************************************)
+  (* for _, ent := range ents {                              *)
+  (*     ent.tpl.WriteLock()                                 *)
+  (* }                                                       *)
+  (* return true                                             *)
+  (***********************************************************)
+
+  (**
+   * Get [own_tuple_locked] for each element in [ents].
+   * Give [Hptuple] (proof of [ptuple_auth]) and [Hlen] to txn, and keep the remaining.
+   * Should convert [ptuple_auth]s from [big_sepL] into [big_sepM].
+   *)
+Admitted.
+
+End heap.
