src/program_proof/mvcc/wrbuf_repr.v
@@ -1,0 +1,47 @@
+From Perennial.program_proof.mvcc Require Import wrbuf_prelude.
+
+Section repr.
+Context `{!heapGS Σ}.
+
+Definition own_wrbuf_xtpls (wrbuf : loc) (mods : dbmap) : iProp Σ :=
+  ∃ (entsS : Slice.t) (ents : list wrent),
+    "Hents"   ∷ wrbuf ↦[WrBuf :: "ents"] (to_val entsS) ∗
+    "HentsS"  ∷ slice.is_slice entsS (structTy WrEnt) 1 (wrent_to_val <$> ents) ∗
+    "%HNoDup" ∷ ⌜NoDup ents.*1.*1.*1⌝ ∗
+    "%Hmods"  ∷ ⌜mods = (list_to_map (wrent_to_key_dbval <$> ents))⌝.
+
+Definition own_wrbuf
+           (wrbuf : loc) (mods : dbmap) (tpls : gmap u64 loc)
+  : iProp Σ :=
+  ∃ (entsS : Slice.t) (ents : list wrent),
+    "Hents"   ∷ wrbuf ↦[WrBuf :: "ents"] (to_val entsS) ∗
+    "HentsS"  ∷ slice.is_slice entsS (structTy WrEnt) 1 (wrent_to_val <$> ents) ∗
+    "%HNoDup" ∷ ⌜NoDup ents.*1.*1.*1⌝ ∗
+    "%Hmods"  ∷ ⌜mods = (list_to_map (wrent_to_key_dbval <$> ents))⌝ ∗
+    "%Htpls"  ∷ ⌜tpls = (list_to_map (wrent_to_key_tpl <$> ents))⌝.
+
+End repr.
+
+#[global]
+Hint Extern 1 (environments.envs_entails _ (own_wrbuf_xtpls _ _)) => unfold own_wrbuf_xtpls : core.
+#[global]
+Hint Extern 1 (environments.envs_entails _ (own_wrbuf _ _ _)) => unfold own_wrbuf : core.
+
+Section lemma.
+Context `{!heapGS Σ}.
+
+Lemma own_wrbuf_mods_tpls_dom wrbuf mods tpls :
+  own_wrbuf wrbuf mods tpls -∗
+  ⌜dom mods = dom tpls⌝.
+Proof.
+  iIntros "Hwrbuf".
+  iNamed "Hwrbuf".
+  iPureIntro.
+  rewrite Hmods Htpls.
+  do 2 rewrite dom_list_to_map_L.
+  unfold wrent_to_key_dbval, wrent_to_key_tpl.
+  f_equal.
+  by do 2 rewrite -list_fmap_compose.
+Qed.
+
+End lemma.
