src/program_proof/mvcc/wrbuf_update_tuples.v
@@ -1,0 +1,33 @@
+From Perennial.program_proof.mvcc Require Import
+     wrbuf_prelude wrbuf_repr
+     tuple_repr tuple_append_version tuple_kill_version.
+
+Section heap.
+Context `{!heapGS Σ, !mvcc_ghostG Σ}.
+
+(*****************************************************************)
+(* func (wrbuf *WrBuf) UpdateTuples(tid uint64)                  *)
+(*****************************************************************)
+Theorem wp_wrbuf__UpdateTuples wrbuf (tid : u64) mods tpls γ :
+  {{{ own_wrbuf wrbuf mods tpls ∗ own_tuples_updated (int.nat tid) mods tpls γ }}}
+    WrBuf__UpdateTuples #wrbuf #tid
+  {{{ RET #(); own_wrbuf_xtpls wrbuf mods }}}.
+Proof.
+  iIntros (Φ) "Hwrbuf HΦ".
+  wp_call.
+  iNamed "Hwrbuf".
+
+  (***********************************************************)
+  (* ents := wrbuf.ents                                      *)
+  (* for _, ent := range ents {                              *)
+  (*     tpl := ent.tpl                                      *)
+  (*     if ent.wr {                                         *)
+  (*         tpl.AppendVersion(tid, ent.val)                 *)
+  (*     } else {                                            *)
+  (*         tpl.KillVersion(tid)                            *)
+  (*     }                                                   *)
+  (* }                                                       *)
+  (***********************************************************)
+Admitted.
+
+End heap.
